\documentclass[11pt,a4paper]{article}
\usepackage[utf8]{inputenc}
\usepackage[english]{babel}
\usepackage{graphicx}
\usepackage{multicol}
\usepackage{amsmath}
\usepackage{hyperref}
\usepackage{amsthm}
\theoremstyle{definition}
\newtheorem{definition}{Definition}
\newtheorem{ex}{Example}
\setlength{\columnsep}{1cm}

 
\begin{document}
\author{Ibrahim Abou Elenein}
\title{Lecture 1 Summary}
\date {\today}
\maketitle
\section{Energy and Power}

\subsection{Energy}

\begin{multicols}{2}
    \textbf{ \ Continuous} 
    \begin{equation}
        E_\infty= \int ^{\infty} _{- \infty} |x(t)|^2 dt 
    \end{equation}
    
    \columnbreak
    
    \textbf{ \  Discrete}
    \begin{equation}
        E_\infty= \sum ^{\infty} _{- \infty} |x[n[|^2
    \end{equation}
\end{multicols}
\subsection{Power}
\subsubsection{For non Periodic Signals }
\begin{multicols}{2}
    
    \textbf{ \ Continuous} 
    \begin{equation}
        P_{\infty} = \displaystyle \lim _{T \to \infty} \frac{1}{2T} \int 
        _{-T} ^{T} |x(t)|^2 dt
    \end{equation}
    
    \columnbreak
    
    \textbf{ \  Discrete}
    \[
        P_{\infty} = \displaystyle \lim _{N \to \infty} \frac{1}{2N+1} \sum 
        _{-N} ^{N} |x[n]|^2 
        \]
\end{multicols}
\subsubsection{For Periodic} 
\[
    P = \frac{1}{T_o} \int_{\frac{-T_o}{2}} ^{\frac{T_o}{2}} |x_p(t)|^2 dt
\]
    where $T_o$ is The Fundamental Period
    
\section{Signal Decomposition}    
\[
    x(t) = Ev{x(t)} + Od{x(t)}
\]
\textbf{With} \\ 

\begin{multicols}{2}
    \[
        Ev \{x(t)\} = \frac{1}{2}[x(t) + x(-t)]
    \]
    
    \columnbreak
    
    \[
        Od \{x(t)\} = \frac{1}{2}[x(t) - x(-t)]
    \]
    
\end{multicols}
\section{Notes}
\begin{itemize}
    \item  A Power Signal is signal its power is finite 
    \item  An Energy Signal is signal its energy is finite 
\end{itemize}
\subsection{From Euler Formula}
\[
    e^{jx} = \cos x + j \sin x \ 
\]
\[
    |e^{jx}| = |\cos x + j \sin x| = \sqrt{\cos^2 x + \sin^2 x} = 1
\]

\subsection{Unit step function}

\[
    u(t) = \begin{cases}
        0, & \text{$t < 0$} \\ 
        1, & \text{$t > 0$}
    \end{cases}
\]
\[
    | f(t)u(t)| = f(t)  \ \  \ \  \   \  0 < t < \infty   
\]
\subsection{Geometric Series}
\[
    a + ar + ar^2 + \dots +ar^n = \displaystyle \sum_{k = 0} ^{n} ar^k = a(\frac{1 - r^{n + 1}}{1 -r}) 
\]
\[
    a + ar + ar^2 + \dots = \displaystyle \sum _{k = 0} ^{\infty} ar^k = \frac{a}{1 - r}
\  \  \  \ for  \ \ |r| < 1 
\]
\subsection{Series}
\[  
    \displaystyle \sum _{i = 1} ^{n} c = n.c
\]
\[  
    \displaystyle \sum _{n = 0} ^{N} c = (N + 1 ).c
\]
\[
    \displaystyle \sum _{n = -N} ^{N} c = \sum _{n = 0}^{2N} c = c (2N + 1) \ 
\]
Shifting by adding the upper and lower bound by N

\[
    \displaystyle \sum _{i = 1} ^n i = \frac{n(n+1)}{2}
\]
\[
    \displaystyle \sum _{i = 1} ^n i^2 = \frac{n(n+1)(2n+1)}{6}
\]

\end{document}
