\documentclass[11pt,a4paper]{article}
\usepackage[utf8]{inputenc}
\usepackage[english]{babel}
\usepackage{graphicx}
\usepackage{multicol}
\usepackage{amsmath}
\usepackage{hyperref}
\usepackage{amsthm}
\theoremstyle{definition}
\newtheorem{definition}{Definition}
\newtheorem{ex}{Example}
\setlength{\columnsep}{1cm}


\begin{document}
\author{\textbf{Ibrahim Abou Elenein}}
\title{\textbf{Properties of CT Fourier Series}}
\date {\today}
\maketitle
\section{Linearity}
Let 
\[
    x(t) \xrightarrow{\mathcal{F}\mathcal{S}} a_k
\]
\[
    y(t) \xrightarrow{\mathcal{F}\mathcal{S}} b_k
\]
two periodic signals with period $T$, then 
\[
    z(t) = Ax(t) + By(t) \xrightarrow{\mathcal{F}\mathcal{S}} c_k = Aa_k + Bb_k
\]
\textbf{Proof}
\[
    c_k = \frac{1}{T} \int_T z(t)e^{-jk\omega_ot} dt 
    = \frac{1}{T} \int_T [Ax(t) + By(t)]e^{-jk\omega_ot} dt
\]
\[
    = A \frac{1}{T} \int_T x(t)e^{-jk\omega_ot} dt + B \frac{1}{T} \int_T y(t) e^{-jk\omega_ot} dt
\]
\[
    = Aa_k+ Ba_k
\]
\section{Time Shifting}
Let 
\[
    x(t) \xrightarrow{\mathcal{F}\mathcal{S}} a_k
\]
Then 
\[
    x(t-t_o) \xrightarrow{\mathcal{F}\mathcal{S}} b_k = e^{-jk\omega_ot_o}a_k = e^{jk(2\frac{\pi}{T})t_0} a_k 
\]
\textbf{Note} $|b_k| = |a_k| $\\


\textbf{Proof}
\[
    b_k = \frac{1}{T} \int_T x(t-t_0) e^{-jk\omega_ot} dt \stackrel{\tau=t-t_o}{=} \frac{1}{T} \int_T 
    x(\tau) e^{-jk\omega_o(\tau+t_o)} d\tau
\]
\[
    = e^{-jk\omega_ot_o}  \underbrace{\frac{1}{T}\int_T x(\tau) e^{-jk\omega_o\tau} d\tau}_{a_k} = e^{-jk\omega_ot_o} a_k
\]
\section{Time Scaling}
\[
    t \Rightarrow \alpha t , \ \ \  \alpha > 0
\]
\begin{enumerate}
    \item period changes $T \rightarrow \frac{T}{\alpha} $
    \item fundamental frequency changes $\omega_o \rightarrow \alpha \omega_o $
\end{enumerate}
Fourier Series representation
\[
    \displaystyle x(\alpha t) = \sum_{k=-\infty}^{\infty} a_k e^{jk(\frac{\alpha 2 \pi}{T})t} =
    \sum_{k=-\infty}^{\infty} a_k e^{jk(\alpha \omega_o)t}
\]
\section{Differentiation}
Let 
\[
    x(t) \xrightarrow{\mathcal{F}\mathcal{S}} a_k
\]
Then 
\[
    \dfrac{dx(t)}{dt} = jk\omega_o a_k
\]
\section{Multiplication}
Let 
\[
    x(t) \xrightarrow{\mathcal{F}\mathcal{S}} a_k
\]
\[
    y(t) \xrightarrow{\mathcal{F}\mathcal{S}} b_k
\]
\[
    z(t) = x(t)y(t) \xrightarrow{\mathcal{F}\mathcal{S}} c_k = \sum_{i=-\infty}^{\infty} a_ib_{k-i} \Rightarrow
    \text{discrete-time convloution of} a_k \ \text{and} \ b_k
\]
\[
    c_k = a_k * b_k
\]
\section{Parseval's Relation}
Let 
\[
    x(t) \xrightarrow{\mathcal{F}\mathcal{S}} a_k
\]
Then 
\[
    \boxed{\frac{1}{T} \int_T |x(t)|^2 dt = \sum_{k=-\infty}^{\infty}|a_k|^2 }
\]
Hence Average total power of the signal is sum of the average powers in all of harmonic components.
\section{Time Reversal}
Let 
\[
    x(t) \xrightarrow{\mathcal{F}\mathcal{S}} a_k
\]
Then 
\[
    x(-t) \xrightarrow{\mathcal{F}\mathcal{S}} b_k = a_{-k}
\]
\textbf{Proof}
\[  
    x(t) = \sum_{k=-\infty}^{\infty} a_k e^{jk\omega_ot}, \Longrightarrow x(-t)= \sum_{k=-\infty}^{\infty} a_k e^{-jk\omega_ot}
\]
\[
    \displaystyle \stackrel{k=-m}{=}  \sum_{m=-\infty}^{\infty} \ a_{-m} e^{jm\omega_ot}
\]

\section{Conjugation and Conjugate Symmetry}
Let 
\[
    x(t) \xrightarrow{\mathcal{F}\mathcal{S}} a_k
\]
Then 
\[
    x^*(t) \xrightarrow{\mathcal{F}\mathcal{S}} a^*_{-k}
\]
\begin{itemize}
    \item If $x(t) = x^*(t) \Rightarrow a_k = a^*_{-k}  \Longrightarrow  x(t) \ \text{real}$
    \item If $x(t) = -x^*(t) \Rightarrow a_k = -a^*_{-k}  \Longrightarrow  x(t) \ \text{img}$

\end{itemize}
\section{Summary}
Let 
\[
    x(t) \xrightarrow{\mathcal{F}\mathcal{S}} a_k
\]
\[
    y(t) \xrightarrow{\mathcal{F}\mathcal{S}} b_k
\]
\begin{enumerate}
    \item Linearity

        \[
            Ax(t) + By(t) \xrightarrow{\mathcal{F}\mathcal{S}} Aa_k + Bb_k
        \]
    \item Time Shift
\[
    x(t-t_o) \xrightarrow{\mathcal{F}\mathcal{S}} a_k e^{-jk\omega_ot_o}
\]
\item Time Scale
\[
    x(\alpha t) \xrightarrow{\mathcal{F}\mathcal{S}} a_k 
\]
\item Differentiation
\[
    \dfrac{dx(t)}{dt} \xrightarrow{\mathcal{F}\mathcal{S}} jk\omega_o a_k
\]
\item Integration
    \[
        \int_{-\infty}^t x(\tau)d\tau \xrightarrow{\mathcal{F}\mathcal{S}} 
        \frac{a_k}{jk\omega_o}
    \]
\item Convolution 
    \[
        x(t)*y(t) \xrightarrow{\mathcal{F}\mathcal{S}} Ta_kb_k
    \]
\item Multiplication
    \[
        x(t)y(t) \xrightarrow{\mathcal{F}\mathcal{S}} a_k*b_k
    \]
\end{enumerate}
\section{Notes}
\begin{itemize}
    \item if $x(t)$ is real \& even $\Rightarrow a_k$ is real \& even   
    \item if $x(t)$ is real \& odd $\Rightarrow a_k$ is pure \& odd.
\end{itemize}
\end{document}
